Experiment with repeati_blocks more...

code/experimental/sha2/Hacl.Impl.SHA2_256.fst
@@ -256,45 +256,47 @@ let shuffle hash wsTable =
   let spec h = Spec.shuffle_core Spec.SHA2_256 h.[|wsTable|] in
   loop1 h0 (size (Spec.size_kTable Spec.SHA2_256)) hash spec
   (fun i ->
-    (admit(); Loops.unfold_repeati (Spec.size_kTable Spec.SHA2_256) (spec h0) h0.[|wsTable|] (v i));
+    Loops.unfold_repeati (Spec.size_kTable Spec.SHA2_256) (spec h0) h0.[|hash|] (v i);
     shuffle_core hash wsTable i)
 
 
 val compress: hash:hash_wp -> block:block_wp ->
   Stack unit
   (requires (fun h -> live h hash /\ live h block /\ disjoint hash block))
-  (ensures  (fun h0 _ h1 -> modifies1 hash h0 h1))
-                       (* /\ h1.[|hash|] == Spec.compress Spec.SHA2_256 h0.[|block|] h0.[|hash|])) *)
+  (ensures  (fun h0 _ h1 -> modifies1 hash h0 h1
+                       /\ h1.[|hash|] == Spec.compress Spec.SHA2_256 h0.[|block|] h0.[|hash|]))
+
+#reset-options "--z3rlimit 150"
 
 let compress hash block =
+  (**) let h0 = ST.get () in
   push_frame();
   let wsTable = create (size (Spec.size_kTable Spec.SHA2_256)) (u32 0) in
-  let hash0 = create (size Spec.size_hash_w) (u32 0) in
+  let hash1 = create (size Spec.size_hash_w) (u32 0) in
   ws wsTable block;
-  copy hash0 hash;
-  shuffle hash wsTable;
-  let h0 = ST.get () in
-  loop_nospec #h0 (size Spec.size_hash_w) hash
-  (fun i ->
-    let x0 = hash0.(i) in
-    let x1 = hash.(i) in
-    hash.(i) <- x0 +. x1);
+  copy hash1 hash;
+  shuffle hash1 wsTable;
+  [@inline_let]
+  (**) let f = (fun x0 x1 -> add_mod #U32 #SEC x0 x1) in
+  map2T (size Spec.size_hash_w) hash f hash hash1;
+  (**) let h5 = ST.get () in
+  (**) Seq.eq_intro (h5.[|hash|]) (Spec.compress Spec.SHA2_256 h0.[|block|] h0.[|hash|]);
   pop_frame ()
 
 
 val truncate: hash:lbuffer uint8 (size (Spec.size_hash Spec.SHA2_256)) -> hw:hash_wp ->
   Stack unit
   (requires (fun h -> live h hash /\ live h hw /\ disjoint hash hw))
-  (ensures  (fun h0 _ h1 -> modifies1 hash h0 h1))
-                       (* /\ h1.[|hash|] == Spec.truncate Spec.SHA2_256 h0.[|hw|])) *)
+  (ensures  (fun h0 _ h1 -> modifies1 hash h0 h1
+                       /\ h1.[|hash|] == Spec.truncate Spec.SHA2_256 h0.[|hw|]))
 
 let truncate hash hw =
-  let h0 = ST.get () in
-  salloc_nospec h0 (size Spec.size_hash_w *. size (Spec.size_word Spec.SHA2_256)) (u8 0) (Ghost.hide (loc hash))
-  (fun hash_full ->
-    uints_to_bytes_be (size Spec.size_hash_w) hash_full hw;
-    let hash_final = sub hash_full (size 0) (size (Spec.size_hash Spec.SHA2_256)) in
-    copy hash hash_final)
+  push_frame ();
+  let hash_full = create (size Spec.size_hash_w *. size (Spec.size_word Spec.SHA2_256)) (u8 0) in
+  uints_to_bytes_be (size Spec.size_hash_w) hash_full hw;
+  let hash_final = sub hash_full (size 0) (size (Spec.size_hash Spec.SHA2_256)) in
+  copy hash hash_final;
+  pop_frame ()
 
 
 (* Definition of the function returning the number of padding blocks for a single input block *)
@@ -302,6 +304,7 @@ let number_blocks_padding (len:size_t{v len <= Spec.size_block Spec.SHA2_256}) :
   Tot (r:size_t{v r == Spec.number_blocks_padding Spec.SHA2_256 (v len)}) =
   if len <. (size (Spec.size_block Spec.SHA2_256) -. 8ul) then 1ul else 2ul
 
+#reset-options "--z3rlimit 150 --max_fuel 0"
 
 (* Definition of the padding function for a single input block *)
 val pad:
@@ -313,8 +316,8 @@ val pad:
                /\ v len + uint_v prev <= Spec.max_input Spec.SHA2_256} ->
   Stack unit
   (requires (fun h -> live h blocks /\ live h last /\ disjoint blocks last))
-  (ensures  (fun h0 _ h1 -> modifies1 blocks h0 h1))
-
+  (ensures  (fun h0 _ h1 -> modifies1 blocks h0 h1
+                       /\ h1.[|blocks|] == Spec.pad Spec.SHA2_256 (v prev) (v len) (as_seq #MUT #uint8 #len h0 last)))
 let pad blocks prev last len =
   let nr = number_blocks_padding len in
   // Create the padding and copy the partial block inside
@@ -329,20 +332,22 @@ let pad blocks prev last len =
   let tlen = prev +. (to_u64 len) in
   let tlenbits = tlen *. (u64 8) in
   let encodedlen = sub blocks (nr *. size (Spec.size_block Spec.SHA2_256) -. 8ul) 8ul in
-  uint_to_bytes_be encodedlen tlenbits
+  uint_to_bytes_be encodedlen tlenbits;
+  admit()
 
 
 val update_block: hash:hash_wp -> block:block_p ->
   Stack unit
   (requires (fun h -> live h hash /\ live h block /\ disjoint hash block))
-  (ensures  (fun h0 _ h1 -> modifies1 hash h0 h1))
+  (ensures  (fun h0 _ h1 -> modifies1 hash h0 h1
+                       /\ h1.[|hash|] == Spec.update_block Spec.SHA2_256 h0.[|block|] h0.[|hash|]))
 
 let update_block hash block =
-  let h0 = ST.get () in
-  salloc_nospec h0 (size Spec.size_block_w) (u32 0) (Ghost.hide (loc hash))
-  (fun blockw ->
-    uints_from_bytes_be blockw block;
-    compress hash blockw)
+  push_frame ();
+  let blockw = create (size Spec.size_block_w) (u32 0) in
+  uints_from_bytes_be blockw block;
+  compress hash blockw;
+  pop_frame ()
 
 
 val init: hash:hash_wp ->
@@ -363,21 +368,56 @@ val update_last:
                /\ v len + uint_v prev <= Spec.max_input Spec.SHA2_256} ->
   Stack unit
   (requires (fun h -> live h hash /\ live h last /\ disjoint hash last))
-  (ensures  (fun h0 _ h1 -> modifies1 hash h0 h1))
+  (ensures  (fun h0 _ h1 -> modifies1 hash h0 h1
+                       /\ h1.[|hash|] == Spec.update_last Spec.SHA2_256 (v prev) (v len) (as_seq #MUT #uint8 #len h0 last) (as_seq h0 hash)))
 
 let update_last hash prev last len =
-  let h0 = ST.get () in
-  salloc_nospec h0 (2ul *. size (Spec.size_block Spec.SHA2_256)) (u8 0) (Ghost.hide (loc hash))
-  (fun blocks ->
-    pad blocks prev last len;
-    let block0 = sub blocks (size 0) (size (Spec.size_block Spec.SHA2_256)) in
-    let block1 = sub blocks (size (Spec.size_block Spec.SHA2_256)) (size (Spec.size_block Spec.SHA2_256)) in
-    if number_blocks_padding len =. 1ul then (
-      update_block hash block0)
-    else (
-      update_block hash block0;
-      update_block hash block1))
+  push_frame ();
+  let blocks = create (2ul *. size (Spec.size_block Spec.SHA2_256)) (u8 0) in
+  pad blocks prev last len;
+  let block0 = sub blocks (size 0) (size (Spec.size_block Spec.SHA2_256)) in
+  let block1 = sub blocks (size (Spec.size_block Spec.SHA2_256)) (size (Spec.size_block Spec.SHA2_256)) in
+  if number_blocks_padding len =. 1ul then (
+     update_block hash block0)
+  else (
+    update_block hash block0;
+    update_block hash block1);
+  pop_frame ()
 
+
+(* Definition of the single block update function *)
+let spec_update_block (p:Spec.alg) (len:size_nat) (i:size_nat{i < len / Spec.size_block p}) (block:Lib.ByteSequence.lbytes (Spec.size_block p)) (hash:Spec.hash_w p): Tot (hf:Spec.hash_w p{hf == Spec.update_block p block hash}) =
+  let bw = Lib.ByteSequence.uints_from_bytes_be block in
+  Spec.compress p bw hash
+
+(* Definition of the function for the partial block compression *)
+let spec_update_last
+  (p:Spec.alg)
+  (flen: size_nat)
+  (i: size_nat{i = flen % Spec.size_block p})
+  (rlen:nat{rlen <= Spec.size_block p /\ rlen + (i * Spec.size_block p) <= Spec.max_input p})
+  (last:Lib.ByteSequence.lbytes rlen)
+  (hash:Spec.hash_w p):
+  Tot (Spec.hash_w p) =
+
+  let prev = i * Spec.size_block p in
+  let blocks = Spec.pad p i rlen last in
+  if Spec.number_blocks_padding p rlen = 1 then
+    Spec.update_block p blocks hash
+  else (
+    let block1 = Lib.Sequence.sub blocks 0 (Spec.size_block p) in
+    let block2 = Lib.Sequence.sub blocks (Spec.size_block p) (Spec.size_block p) in
+    let hash = Spec.update_block p block1 hash in
+    Spec.update_block p block2 hash)
+
+
+(* Definition of the update function *)
+let spec_update (p:Spec.alg) (input:Lib.Sequence.seq uint8) (hash:Spec.hash_w p): Tot (Spec.hash_w p) =
+  admit();
+  assume(Lib.Sequence.length input <= max_size_t);
+  Lib.Sequence.repeati_blocks #uint8 #(hash:Spec.hash_w p) (Spec.size_block p) input
+    (spec_update_block p (Lib.Sequence.length input))
+    (spec_update_last p (Lib.Sequence.length input)) hash
 
 val update:
     hash: hash_wp
@@ -386,20 +426,25 @@ val update:
                /\ v len <= Spec.max_input Spec.SHA2_256} ->
   Stack unit
   (requires (fun h -> live h hash /\ live h input /\ disjoint hash input))
-  (ensures  (fun h0 _ h1 -> modifies1 hash h0 h1))
+  (ensures  (fun h0 _ h1 -> modifies1 hash h0 h1
+                       /\ h1.[|hash|] == Spec.update Spec.SHA2_256 (as_seq #MUT #uint8 #len h0 input) h0.[|hash|]))
 
 let update hash input len =
+  admit();
   let h0 = ST.get() in
-  loopi_blocks_nospec (size (Spec.size_block Spec.SHA2_256)) len input
-    (fun i block hash -> update_block hash block)
-    (fun i len last hash -> update_last hash (to_u64 i *. u64 (Spec.size_block Spec.SHA2_256)) last len)
+  loopi_blocks (size (Spec.size_block Spec.SHA2_256)) len input
+    (spec_update_block Spec.SHA2_256 (v len))
+    (spec_update_last Spec.SHA2_256 (v len))
+    (fun i block hash -> update_block hash len)
+    (fun i len last hash -> update_last hash len len last)
     hash
 
 
 val finish: hash:lbuffer uint8 (size (Spec.size_hash Spec.SHA2_256)) -> hw:hash_wp ->
   Stack unit
   (requires (fun h -> live h hash /\ live h hw /\ disjoint hash hw))
-  (ensures  (fun h0 _ h1 -> modifies1 hash h0 h1))
+  (ensures  (fun h0 _ h1 -> modifies1 hash h0 h1
+                       /\ h1.[|hash|] == Spec.finish Spec.SHA2_256 h0.[|hw|]))
 
 let finish hash hw = truncate hash hw
 
@@ -410,12 +455,14 @@ val hash:
   -> len: size_t{length input == v len /\ v len <= Spec.max_input Spec.SHA2_256} ->
   Stack unit
   (requires (fun h -> live h output /\ live h input /\ disjoint output input))
-  (ensures  (fun h0 _ h1 -> modifies1 output h0 h1))
+  (ensures  (fun h0 _ h1 -> modifies1 output h0 h1
+                       /\ h1.[|output|] == Spec.hash Spec.SHA2_256 (as_seq #MUT #uint8 #len h0 input)))
 
 let hash output input len =
   let h0 = ST.get () in
-  salloc_nospec h0 (size Spec.size_hash_w) (u32 0) (Ghost.hide (loc output))
-  (fun hash ->
-    init hash;
-    update hash input len;
-    finish output hash)
+  push_frame ();
+  let hash = create (size Spec.size_hash_w) (u32 0) in
+  init hash;
+  update hash input len;
+  finish output hash;
+  pop_frame ()
